Add placeholder rewrite rules for rewriting after bounds
Currently, there aren't any interesting rewrite rules in the lists, but
this allows us to move rewrite rules that depend on cast behavior to
after bounds analysis.

Unfortunately, it takes a lot of time to build from Rewriter.v to the
standalone binaries, so it'll probably make sense to inline some stuff
for more rapid development.

Note that we also now have a tactic that does all of the evaluation for
rewrite rules (assuming the right [Arguments] commands have been
issued).

src/Experiments/NewPipeline/Rewriter.v
@@ -5,6 +5,8 @@ Require Import Crypto.Util.ListUtil Coq.Lists.List Crypto.Util.ListUtil.FoldBool
 Require Import Crypto.Util.Option.
 Require Import Crypto.Util.OptionList.
 Require Import Crypto.Util.CPSNotations.
+Require Import Crypto.Util.ZRange.
+Require Import Crypto.Util.ZRange.Operations.
 Require Crypto.Util.PrimitiveProd.
 Require Crypto.Util.PrimitiveHList.
 Require Import Crypto.Experiments.NewPipeline.Language.
@@ -1854,17 +1856,29 @@ Module Compilers.
             ; make_rewriteol (-??) (fun e => (llet v := e in -$v)  when  negb (SubstVarLike.is_var_fst_snd_pair_opp e)) (* inline negation when the rewriter wouldn't already inline it *)
            ].
 
+      Definition arith_with_casts_rewrite_rules : rewrite_rulesT
+        := [make_rewrite (#(@pattern.ident.fst '1 '2) @ (??, ??)) (fun _ _ x y => x)
+            ; make_rewrite (#(@pattern.ident.snd '1 '2) @ (??, ??)) (fun _ x _ y => y)
+            ; make_rewriteo
+                (#pattern.ident.Z_cast @ (#pattern.ident.Z_cast @ ??))
+                (fun r1 r2 x => #(ident.Z_cast r2) @ x  when  ZRange.is_tighter_than_bool (ZRange.normalize r2) (ZRange.normalize r1))].
+
       Definition nbe_dtree'
         := Eval compute in @compile_rewrites ident var pattern.ident (@pattern.ident.arg_types) pattern.Raw.ident (@pattern.ident.strip_types) pattern.Raw.ident.ident_beq (@pattern.ident.type_vars) 100 nbe_rewrite_rules.
       Definition arith_dtree'
         := Eval compute in @compile_rewrites ident var pattern.ident (@pattern.ident.arg_types) pattern.Raw.ident (@pattern.ident.strip_types) pattern.Raw.ident.ident_beq (@pattern.ident.type_vars) 100 (arith_rewrite_rules 0%Z (* dummy val *)).
+      Definition arith_with_casts_dtree'
+        := Eval compute in @compile_rewrites ident var pattern.ident (@pattern.ident.arg_types) pattern.Raw.ident (@pattern.ident.strip_types) pattern.Raw.ident.ident_beq (@pattern.ident.type_vars) 100 arith_with_casts_rewrite_rules.
       Definition nbe_dtree : decision_tree
         := Eval compute in invert_Some nbe_dtree'.
       Definition arith_dtree : decision_tree
         := Eval compute in invert_Some arith_dtree'.
+      Definition arith_with_casts_dtree : decision_tree
+        := Eval compute in invert_Some arith_with_casts_dtree'.
 
       Definition nbe_default_fuel := Eval compute in List.length nbe_rewrite_rules.
       Definition arith_default_fuel := Eval compute in List.length (arith_rewrite_rules 0%Z (* dummy val *)).
+      Definition arith_with_casts_default_fuel := Eval compute in List.length arith_with_casts_rewrite_rules.
 
       Import PrimitiveHList.
       (* N.B. The [combine_hlist] call MUST eta-expand
@@ -1888,10 +1902,16 @@ Module Compilers.
       Definition arith_pr1_rewrite_rules max_const_val := Eval hnf in projT1 (arith_split_rewrite_rules max_const_val).
       Definition arith_pr2_rewrite_rules max_const_val := Eval hnf in projT2 (arith_split_rewrite_rules max_const_val).
       Definition arith_all_rewrite_rules max_const_val := combine_hlist (P:=rewrite_ruleTP) (arith_pr1_rewrite_rules max_const_val) (arith_pr2_rewrite_rules max_const_val).
+      Definition arith_with_casts_split_rewrite_rules := Eval cbv [split_list projT1 projT2 arith_with_casts_rewrite_rules] in split_list arith_with_casts_rewrite_rules.
+      Definition arith_with_casts_pr1_rewrite_rules := Eval hnf in projT1 arith_with_casts_split_rewrite_rules.
+      Definition arith_with_casts_pr2_rewrite_rules := Eval hnf in projT2 arith_with_casts_split_rewrite_rules.
+      Definition arith_with_casts_all_rewrite_rules := combine_hlist (P:=rewrite_ruleTP) (arith_with_casts_pr1_rewrite_rules) arith_with_casts_pr2_rewrite_rules.
       Definition nbe_rewrite_head0 do_again {t} (idc : ident t) : value_with_lets t
         := @assemble_identifier_rewriters nbe_dtree nbe_all_rewrite_rules do_again t idc.
       Definition arith_rewrite_head0 max_const_val do_again {t} (idc : ident t) : value_with_lets t
         := @assemble_identifier_rewriters arith_dtree (arith_all_rewrite_rules max_const_val) do_again t idc.
+      Definition arith_with_casts_rewrite_head0 do_again {t} (idc : ident t) : value_with_lets t
+        := @assemble_identifier_rewriters arith_with_casts_dtree arith_with_casts_all_rewrite_rules do_again t idc.
 
       Section fancy.
         Context (invert_low invert_high : Z (*log2wordmax*) -> Z -> option Z).
@@ -2067,18 +2087,32 @@ Z.mul @@ (?x >> 128, ?y >> 128)             --> mulhh @@ (x, y)
                   ((#pattern.ident.Z_shiftr @ ?? @ #?ℤ) * (#pattern.ident.Z_shiftr @ ?? @ #?ℤ))
                   (fun x offset1 y offset2 => let s := (2*offset1)%Z in #(ident.fancy_mulhh s) @ (x, y)  when  offset1 =? offset2)
             ].
+        Definition fancy_with_casts_rewrite_rules : rewrite_rulesT
+          := [].
+
         Definition fancy_dtree'
           := Eval compute in @compile_rewrites ident var pattern.ident (@pattern.ident.arg_types) pattern.Raw.ident (@pattern.ident.strip_types) pattern.Raw.ident.ident_beq (@pattern.ident.type_vars) 100 fancy_rewrite_rules.
         Definition fancy_dtree : decision_tree
           := Eval compute in invert_Some fancy_dtree'.
+        Definition fancy_with_casts_dtree'
+          := Eval compute in @compile_rewrites ident var pattern.ident (@pattern.ident.arg_types) pattern.Raw.ident (@pattern.ident.strip_types) pattern.Raw.ident.ident_beq (@pattern.ident.type_vars) 100 fancy_with_casts_rewrite_rules.
+        Definition fancy_with_casts_dtree : decision_tree
+          := Eval compute in invert_Some fancy_with_casts_dtree'.
         Definition fancy_default_fuel := Eval compute in List.length fancy_rewrite_rules.
+        Definition fancy_with_casts_default_fuel := Eval compute in List.length fancy_with_casts_rewrite_rules.
         Import PrimitiveHList.
         Definition fancy_split_rewrite_rules := Eval cbv [split_list projT1 projT2 fancy_rewrite_rules] in split_list fancy_rewrite_rules.
         Definition fancy_pr1_rewrite_rules := Eval hnf in projT1 fancy_split_rewrite_rules.
         Definition fancy_pr2_rewrite_rules := Eval hnf in projT2 fancy_split_rewrite_rules.
         Definition fancy_all_rewrite_rules := combine_hlist (P:=rewrite_ruleTP) fancy_pr1_rewrite_rules fancy_pr2_rewrite_rules.
+        Definition fancy_with_casts_split_rewrite_rules := Eval cbv [split_list projT1 projT2 fancy_with_casts_rewrite_rules] in split_list fancy_with_casts_rewrite_rules.
+        Definition fancy_with_casts_pr1_rewrite_rules := Eval hnf in projT1 fancy_with_casts_split_rewrite_rules.
+        Definition fancy_with_casts_pr2_rewrite_rules := Eval hnf in projT2 fancy_with_casts_split_rewrite_rules.
+        Definition fancy_with_casts_all_rewrite_rules := combine_hlist (P:=rewrite_ruleTP) fancy_with_casts_pr1_rewrite_rules fancy_with_casts_pr2_rewrite_rules.
         Definition fancy_rewrite_head0 do_again {t} (idc : ident t) : value_with_lets t
           := @assemble_identifier_rewriters fancy_dtree fancy_all_rewrite_rules do_again t idc.
+        Definition fancy_with_casts_rewrite_head0 do_again {t} (idc : ident t) : value_with_lets t
+          := @assemble_identifier_rewriters fancy_with_casts_dtree fancy_with_casts_all_rewrite_rules do_again t idc.
       End fancy.
     End with_var.
     Module RewriterPrintingNotations.
@@ -2103,193 +2137,150 @@ Z.mul @@ (?x >> 128, ?y >> 128)             --> mulhh @@ (x, y)
       Notation "x <- 'type.try_make_transport_cps' t1 t2 ; f" := (type.try_make_transport_cps t1 t2 (fun y => match y with Some x => f | None => None end)) (at level 70, t1 at next level, t2 at next level, right associativity, format "'[v' x  <-  'type.try_make_transport_cps'  t1  t2 ; '/' f ']'").
       Notation "x <- 'base.try_make_transport_cps' t1 t2 ; f" := (base.try_make_transport_cps t1 t2 (fun y => match y with Some x => f | None => None end)) (at level 70, t1 at next level, t2 at next level, right associativity, format "'[v' x  <-  'base.try_make_transport_cps'  t1  t2 ; '/' f ']'").
     End RewriterPrintingNotations.
+
+    Ltac make_rewrite_head1 rewrite_head0 pr2_rewrite_rules :=
+      (eval cbv -[pr2_rewrite_rules
+                    base.interp base.try_make_transport_cps
+                    type.try_make_transport_cps type.try_transport_cps
+                    pattern.type.unify_extracted_cps
+                    Let_In Option.sequence Option.sequence_return
+                    UnderLets.splice UnderLets.to_expr
+                    Compile.option_bind' pident_unify_unknown invert_bind_args_unknown Compile.normalize_deep_rewrite_rule
+                    Compile.reflect UnderLets.reify_and_let_binds_base_cps Compile.reify Compile.reify_and_let_binds_cps
+                    Compile.value'
+                    SubstVarLike.is_var_fst_snd_pair_opp
+                 ] in rewrite_head0).
+    Ltac timed_make_rewrite_head1 rewrite_head0 pr2_rewrite_rules :=
+      constr:(ltac:(time (idtac; let v := make_rewrite_head1 rewrite_head0 pr2_rewrite_rules in exact v))).
+    Ltac make_rewrite_head2 rewrite_head1 pr2_rewrite_rules :=
+      (eval cbv [id
+                   pr2_rewrite_rules
+                   projT1 projT2
+                   cpsbind cpscall cps_option_bind cpsreturn
+                   PrimitiveProd.Primitive.fst PrimitiveProd.Primitive.snd
+                   pattern.ident.arg_types
+                   Compile.eval_decision_tree
+                   Compile.eval_rewrite_rules
+                   Compile.expr_of_rawexpr
+                   Compile.normalize_deep_rewrite_rule
+                   Compile.option_bind' pident_unify_unknown invert_bind_args_unknown Compile.normalize_deep_rewrite_rule
+                   (*Compile.reflect*)
+                   (*Compile.reify*)
+                   Compile.reveal_rawexpr_cps
+                   Compile.reveal_rawexpr_cps_gen
+                   Compile.rew_should_do_again
+                   Compile.rew_with_opt
+                   Compile.rew_under_lets
+                   Compile.rew_replacement
+                   Compile.rew_is_cps
+                   Compile.rValueOrExpr
+                   Compile.swap_list
+                   Compile.type_of_rawexpr
+                   Compile.value
+                   (*Compile.value'*)
+                   Compile.value_of_rawexpr
+                   Compile.value_with_lets
+                   ident.smart_Literal
+                   type.try_transport_cps
+                   rlist_rect rwhen rwhenl
+                ] in rewrite_head1).
+    Ltac timed_make_rewrite_head2 rewrite_head1 pr2_rewrite_rules :=
+      constr:(ltac:(time (idtac; let v := make_rewrite_head2 rewrite_head1 pr2_rewrite_rules in exact v))).
+    Ltac make_rewrite_head3 rewrite_head2 :=
+      (eval cbn [id
+                   cpsbind cpscall cps_option_bind cpsreturn
+                   Compile.reify Compile.reify_and_let_binds_cps Compile.reflect Compile.value'
+                   Option.sequence Option.sequence_return Option.bind
+                   UnderLets.reify_and_let_binds_base_cps
+                   UnderLets.splice UnderLets.splice_list UnderLets.to_expr
+                   base.interp base.base_interp
+                   base.type.base_beq
+                   type.try_make_transport_cps base.try_make_transport_cps base.try_make_base_transport_cps
+                   Datatypes.fst Datatypes.snd
+                ] in rewrite_head2).
+    Ltac timed_make_rewrite_head3 rewrite_head2 :=
+      constr:(ltac:(time (idtac; let v := make_rewrite_head3 rewrite_head2 in exact v))).
+    Ltac make_rewrite_head rewrite_head0 pr2_rewrite_rules :=
+      let rewrite_head1 := make_rewrite_head1 rewrite_head0 pr2_rewrite_rules in
+      let rewrite_head2 := make_rewrite_head2 rewrite_head1 pr2_rewrite_rules in
+      let rewrite_head3 := make_rewrite_head3 rewrite_head2 in
+      rewrite_head3.
+    Ltac timed_make_rewrite_head rewrite_head0 pr2_rewrite_rules :=
+      let rewrite_head1 := timed_make_rewrite_head1 rewrite_head0 pr2_rewrite_rules in
+      let rewrite_head2 := timed_make_rewrite_head2 rewrite_head1 pr2_rewrite_rules in
+      let rewrite_head3 := timed_make_rewrite_head3 rewrite_head2 in
+      rewrite_head3.
+    Notation make_rewrite_head rewrite_head0 pr2_rewrite_rules
+      := (ltac:(let v := timed_make_rewrite_head rewrite_head0 pr2_rewrite_rules in
+                exact v)) (only parsing).
+
+    (* For reduction *)
+    Local Arguments base.try_make_base_transport_cps _ !_ !_.
+    Local Arguments base.try_make_transport_cps _ !_ !_.
+    Local Arguments type.try_make_transport_cps _ _ _ !_ !_.
+    Local Arguments Option.sequence {A} !v1 v2.
+    Local Arguments Option.sequence_return {A} !v1 v2.
+    Local Arguments Option.bind {A B} !_ _.
+    Local Arguments pattern.Raw.ident.invert_bind_args {t} !_ !_.
+    Local Arguments base.try_make_transport_cps {P} t1 t2 {_} _.
+    Local Arguments type.try_make_transport_cps {base_type _ P} t1 t2 {_} _.
+    Local Arguments base.type.base_beq !_ !_.
+    Local Arguments id / .
+    (* For printing *)
+    Local Arguments option {_}.
+    Local Arguments UnderLets.UnderLets {_ _ _}.
+    Local Arguments expr.expr {_ _ _}.
+    Local Notation ℤ := base.type.Z.
+    Local Notation ℕ := base.type.nat.
+    Local Notation bool := base.type.bool.
+    Local Notation unit := base.type.unit.
+    Local Notation list := base.type.list.
+    Local Notation "x" := (type.base x) (only printing, at level 9).
+
     Section red_fancy.
-      Context (invert_low invert_high : Z (*log2wordmax*) -> Z -> option Z)
+      Context (invert_low invert_high : Z (*log2wordmax*) -> Z -> @option Z)
               {var : type.type base.type -> Type}
               (do_again : forall t : base.type, @expr base.type ident (@Compile.value base.type ident var) (type.base t)
-                                                -> UnderLets.UnderLets base.type ident var (@expr base.type ident var (type.base t)))
+                                                -> @UnderLets.UnderLets base.type ident var (@expr base.type ident var (type.base t)))
               {t} (idc : ident t).
-      Time Let rewrite_head1
-        := Eval cbv -[fancy_pr2_rewrite_rules
-                        base.interp base.try_make_transport_cps
-                        type.try_make_transport_cps type.try_transport_cps
-                        pattern.type.unify_extracted_cps
-                        Let_In Option.sequence Option.sequence_return
-                        UnderLets.splice UnderLets.to_expr
-                        Compile.option_bind' pident_unify_unknown invert_bind_args_unknown Compile.normalize_deep_rewrite_rule
-                        Compile.reflect UnderLets.reify_and_let_binds_base_cps Compile.reify Compile.reify_and_let_binds_cps
-                        Compile.value'
-                        SubstVarLike.is_var_fst_snd_pair_opp
-                     ] in @fancy_rewrite_head0 var invert_low invert_high do_again t idc.
-      (* Finished transaction in 3.395 secs (3.395u,0.s) (successful) *)
-
-      Time Local Definition fancy_rewrite_head2
-        := Eval cbv [id
-                       rewrite_head1 fancy_pr2_rewrite_rules
-                       projT1 projT2
-                       cpsbind cpscall cps_option_bind cpsreturn
-                       PrimitiveProd.Primitive.fst PrimitiveProd.Primitive.snd
-                       pattern.ident.arg_types
-                       Compile.eval_decision_tree
-                       Compile.eval_rewrite_rules
-                       Compile.expr_of_rawexpr
-                       Compile.normalize_deep_rewrite_rule
-                       Compile.option_bind' pident_unify_unknown invert_bind_args_unknown Compile.normalize_deep_rewrite_rule
-                       (*Compile.reflect*)
-                       (*Compile.reify*)
-                       Compile.reveal_rawexpr_cps
-                       Compile.reveal_rawexpr_cps_gen
-                       Compile.rew_should_do_again
-                       Compile.rew_with_opt
-                       Compile.rew_under_lets
-                       Compile.rew_replacement
-                       Compile.rew_is_cps
-                       Compile.rValueOrExpr
-                       Compile.swap_list
-                       Compile.type_of_rawexpr
-                       Compile.value
-                       (*Compile.value'*)
-                       Compile.value_of_rawexpr
-                       Compile.value_with_lets
-                       ident.smart_Literal
-                       type.try_transport_cps
-                       rlist_rect rwhen rwhenl
-                    ] in rewrite_head1.
-      (* Finished transaction in 10.793 secs (10.796u,0.s) (successful) *)
-
-      Local Arguments base.try_make_base_transport_cps _ !_ !_.
-      Local Arguments base.try_make_transport_cps _ !_ !_.
-      Local Arguments type.try_make_transport_cps _ _ _ !_ !_.
-      Local Arguments Option.sequence {A} !v1 v2.
-      Local Arguments Option.sequence_return {A} !v1 v2.
-      Local Arguments Option.bind {A B} !_ _.
-      Local Arguments pattern.Raw.ident.invert_bind_args {t} !_ !_.
-      Local Arguments base.try_make_transport_cps {P} t1 t2 {_} _.
-      Local Arguments type.try_make_transport_cps {base_type _ P} t1 t2 {_} _.
-      Local Arguments base.type.base_beq !_ !_.
-      Local Arguments option {_}.
-      Local Arguments id / .
-      Local Arguments fancy_rewrite_head2 / .
-      Local Arguments UnderLets.UnderLets {_ _ _}.
-      Local Arguments expr.expr {_ _ _}.
-      Local Notation ℤ := base.type.Z.
-      Local Notation ℕ := base.type.nat.
-      Local Notation bool := base.type.bool.
-      Local Notation unit := base.type.unit.
-      Local Notation list := base.type.list.
-      Local Notation "x" := (type.base x) (only printing, at level 9).
 
       Time Definition fancy_rewrite_head
-        := Eval cbn [id
-                       fancy_rewrite_head2
-                       cpsbind cpscall cps_option_bind cpsreturn
-                       Compile.reify Compile.reify_and_let_binds_cps Compile.reflect Compile.value'
-                       Option.sequence Option.sequence_return Option.bind
-                       UnderLets.reify_and_let_binds_base_cps
-                       UnderLets.splice UnderLets.splice_list UnderLets.to_expr
-                       base.interp base.base_interp
-                       base.type.base_beq
-                       type.try_make_transport_cps base.try_make_transport_cps base.try_make_base_transport_cps
-                       Datatypes.fst Datatypes.snd
-                    ] in fancy_rewrite_head2.
-      (* Finished transaction in 1.892 secs (1.891u,0.s) (successful) *)
+        := make_rewrite_head (@fancy_rewrite_head0 var invert_low invert_high do_again t idc) (@fancy_pr2_rewrite_rules).
+      (* Tactic call ran for 0.19 secs (0.187u,0.s) (success)
+         Tactic call ran for 10.297 secs (10.3u,0.s) (success)
+         Tactic call ran for 1.746 secs (1.747u,0.s) (success)
+         Finished transaction in 12.402 secs (12.4u,0.s) (successful) *)
 
       Local Set Printing Depth 1000000.
       Local Set Printing Width 200.
       Import RewriterPrintingNotations.
       (* Redirect "/tmp/fancy_rewrite_head" Print fancy_rewrite_head. *)
     End red_fancy.
+    Section red_fancy_with_casts.
+      Context (invert_low invert_high : Z (*log2wordmax*) -> Z -> @option Z)
+              {var : type.type base.type -> Type}
+              (do_again : forall t : base.type, @expr base.type ident (@Compile.value base.type ident var) (type.base t)
+                                                -> @UnderLets.UnderLets base.type ident var (@expr base.type ident var (type.base t)))
+              {t} (idc : ident t).
+      Time Definition fancy_with_casts_rewrite_head
+        := make_rewrite_head (@fancy_with_casts_rewrite_head0 var (*invert_low invert_high*) do_again t idc) (@fancy_with_casts_pr2_rewrite_rules).
 
+      Local Set Printing Depth 1000000.
+      Local Set Printing Width 200.
+      Import RewriterPrintingNotations.
+      (* Redirect "/tmp/fancy_with_casts_rewrite_head" Print fancy_with_casts_rewrite_head. *)
+    End red_fancy_with_casts.
     Section red_nbe.
       Context {var : type.type base.type -> Type}
               (do_again : forall t : base.type, @expr base.type ident (@Compile.value base.type ident var) (type.base t)
-                                                -> UnderLets.UnderLets base.type ident var (@expr base.type ident var (type.base t)))
+                                                -> @UnderLets.UnderLets base.type ident var (@expr base.type ident var (type.base t)))
               {t} (idc : ident t).
-
-      Time Let rewrite_head1
-        := Eval cbv -[nbe_pr2_rewrite_rules
-                        base.interp base.try_make_transport_cps
-                        type.try_make_transport_cps type.try_transport_cps
-                        pattern.type.unify_extracted_cps
-                        Let_In Option.sequence Option.sequence_return
-                        UnderLets.splice UnderLets.to_expr
-                        Compile.option_bind' pident_unify_unknown invert_bind_args_unknown Compile.normalize_deep_rewrite_rule
-                        Compile.reflect UnderLets.reify_and_let_binds_base_cps Compile.reify Compile.reify_and_let_binds_cps
-                        Compile.value'
-                        SubstVarLike.is_var_fst_snd_pair_opp
-                     ] in @nbe_rewrite_head0 var do_again t idc.
-      (* Finished transaction in 7.035 secs (7.036u,0.s) (successful) *)
-
-      Time Local Definition nbe_rewrite_head2
-        := Eval cbv [id
-                       rewrite_head1 nbe_pr2_rewrite_rules
-                       projT1 projT2
-                       cpsbind cpscall cps_option_bind cpsreturn
-                       PrimitiveProd.Primitive.fst PrimitiveProd.Primitive.snd
-                       pattern.ident.arg_types
-                       Compile.eval_decision_tree
-                       Compile.eval_rewrite_rules
-                       Compile.expr_of_rawexpr
-                       Compile.normalize_deep_rewrite_rule
-                       Compile.option_bind' pident_unify_unknown invert_bind_args_unknown Compile.normalize_deep_rewrite_rule
-                       (*Compile.reflect*)
-                       (*Compile.reify*)
-                       Compile.reveal_rawexpr_cps
-                       Compile.reveal_rawexpr_cps_gen
-                       Compile.rew_should_do_again
-                       Compile.rew_with_opt
-                       Compile.rew_under_lets
-                       Compile.rew_replacement
-                       Compile.rew_is_cps
-                       Compile.rValueOrExpr
-                       Compile.swap_list
-                       Compile.type_of_rawexpr
-                       Compile.value
-                       (*Compile.value'*)
-                       Compile.value_of_rawexpr
-                       Compile.value_with_lets
-                       ident.smart_Literal
-                       type.try_transport_cps
-                       rlist_rect rwhen rwhenl
-                    ] in rewrite_head1.
-      (* Finished transaction in 29.297 secs (29.284u,0.016s) (successful) *)
-
-      Local Arguments base.try_make_base_transport_cps _ !_ !_.
-      Local Arguments base.try_make_transport_cps _ !_ !_.
-      Local Arguments type.try_make_transport_cps _ _ _ !_ !_.
-      Local Arguments Option.sequence {A} !v1 v2.
-      Local Arguments Option.sequence_return {A} !v1 v2.
-      Local Arguments Option.bind {A B} !_ _.
-      Local Arguments pattern.Raw.ident.invert_bind_args {t} !_ !_.
-      Local Arguments base.try_make_transport_cps {P} t1 t2 {_} _.
-      Local Arguments type.try_make_transport_cps {base_type _ P} t1 t2 {_} _.
-      Local Arguments base.type.base_beq !_ !_.
-      Local Arguments option {_}.
-      Local Arguments id / .
-      Local Arguments nbe_rewrite_head2 / .
-      Local Arguments UnderLets.UnderLets {_ _ _}.
-      Local Arguments expr.expr {_ _ _}.
-      Local Notation ℤ := base.type.Z.
-      Local Notation ℕ := base.type.nat.
-      Local Notation bool := base.type.bool.
-      Local Notation unit := base.type.unit.
-      Local Notation list := base.type.list.
-      Local Notation "x" := (type.base x) (only printing, at level 9).
-
       Time Definition nbe_rewrite_head
-        := Eval cbn [id
-                       nbe_rewrite_head2
-                       cpsbind cpscall cps_option_bind cpsreturn
-                       Compile.reify Compile.reify_and_let_binds_cps Compile.reflect Compile.value'
-                       Option.sequence Option.sequence_return Option.bind
-                       UnderLets.reify_and_let_binds_base_cps
-                       UnderLets.splice UnderLets.splice_list UnderLets.to_expr
-                       base.interp base.base_interp
-                       base.type.base_beq
-                       type.try_make_transport_cps base.try_make_transport_cps base.try_make_base_transport_cps
-                       PrimitiveProd.Primitive.fst PrimitiveProd.Primitive.snd Datatypes.fst Datatypes.snd
-                    ] in nbe_rewrite_head2.
-      (* Finished transaction in 1.998 secs (2.u,0.s) (successful) *)
+        := make_rewrite_head (@nbe_rewrite_head0 var do_again t idc) (@nbe_pr2_rewrite_rules).
+      (* Tactic call ran for 0.232 secs (0.235u,0.s) (success)
+         Tactic call ran for 29.061 secs (29.04u,0.004s) (success)
+         Tactic call ran for 1.605 secs (1.604u,0.s) (success)
+         Finished transaction in 31.203 secs (31.183u,0.004s) (successful) *)
 
       Local Set Printing Depth 1000000.
       Local Set Printing Width 200.
@@ -2301,93 +2292,15 @@ Z.mul @@ (?x >> 128, ?y >> 128)             --> mulhh @@ (x, y)
       Context (max_const_val : Z)
               {var : type.type base.type -> Type}
               (do_again : forall t : base.type, @expr base.type ident (@Compile.value base.type ident var) (type.base t)
-                                                -> UnderLets.UnderLets base.type ident var (@expr base.type ident var (type.base t)))
+                                                -> @UnderLets.UnderLets base.type ident var (@expr base.type ident var (type.base t)))
               {t} (idc : ident t).
 
-      Time Let rewrite_head1
-        := Eval cbv -[arith_pr2_rewrite_rules
-                        base.interp base.try_make_transport_cps
-                        type.try_make_transport_cps type.try_transport_cps
-                        pattern.type.unify_extracted_cps
-                        Let_In Option.sequence Option.sequence_return
-                        UnderLets.splice UnderLets.to_expr
-                        Compile.option_bind' pident_unify_unknown invert_bind_args_unknown Compile.normalize_deep_rewrite_rule
-                        Compile.reflect UnderLets.reify_and_let_binds_base_cps Compile.reify Compile.reify_and_let_binds_cps
-                        Compile.value'
-                        SubstVarLike.is_var_fst_snd_pair_opp
-                     ] in @arith_rewrite_head0 var max_const_val do_again t idc.
-      (* Finished transaction in 15.381 secs (15.379u,0.s) (successful) *)
-
-      Time Local Definition arith_rewrite_head2
-        := Eval cbv [id
-                       rewrite_head1 arith_pr2_rewrite_rules
-                       projT1 projT2
-                       cpsbind cpscall cps_option_bind cpsreturn
-                       PrimitiveProd.Primitive.fst PrimitiveProd.Primitive.snd
-                       pattern.ident.arg_types
-                       Compile.eval_decision_tree
-                       Compile.eval_rewrite_rules
-                       Compile.expr_of_rawexpr
-                       Compile.normalize_deep_rewrite_rule
-                       Compile.option_bind' pident_unify_unknown invert_bind_args_unknown Compile.normalize_deep_rewrite_rule
-                       (*Compile.reflect*)
-                       (*Compile.reify*)
-                       Compile.reveal_rawexpr_cps
-                       Compile.reveal_rawexpr_cps_gen
-                       Compile.rew_should_do_again
-                       Compile.rew_with_opt
-                       Compile.rew_under_lets
-                       Compile.rew_replacement
-                       Compile.rew_is_cps
-                       Compile.rValueOrExpr
-                       Compile.swap_list
-                       Compile.type_of_rawexpr
-                       Compile.value
-                       (*Compile.value'*)
-                       Compile.value_of_rawexpr
-                       Compile.value_with_lets
-                       ident.smart_Literal
-                       type.try_transport_cps
-                       rlist_rect rwhen rwhenl
-                    ] in rewrite_head1.
-      (* Finished transaction in 83.667 secs (83.564u,0.115s) (successful) *)
-
-      Local Arguments base.try_make_base_transport_cps _ !_ !_.
-      Local Arguments base.try_make_transport_cps _ !_ !_.
-      Local Arguments type.try_make_transport_cps _ _ _ !_ !_.
-      Local Arguments Option.sequence {A} !v1 v2.
-      Local Arguments Option.sequence_return {A} !v1 v2.
-      Local Arguments Option.bind {A B} !_ _.
-      Local Arguments pattern.Raw.ident.invert_bind_args {t} !_ !_.
-      Local Arguments base.try_make_transport_cps {P} t1 t2 {_} _.
-      Local Arguments type.try_make_transport_cps {base_type _ P} t1 t2 {_} _.
-      Local Arguments base.type.base_beq !_ !_.
-      Local Arguments option {_}.
-      Local Arguments id / .
-      Local Arguments arith_rewrite_head2 / .
-      Local Arguments UnderLets.UnderLets {_ _ _}.
-      Local Arguments expr.expr {_ _ _}.
-      Local Notation ℤ := base.type.Z.
-      Local Notation ℕ := base.type.nat.
-      Local Notation bool := base.type.bool.
-      Local Notation unit := base.type.unit.
-      Local Notation list := base.type.list.
-      Local Notation "x" := (type.base x) (only printing, at level 9).
-
       Time Definition arith_rewrite_head
-        := Eval cbn [id
-                       arith_rewrite_head2
-                       cpsbind cpscall cps_option_bind cpsreturn
-                       Compile.reify Compile.reify_and_let_binds_cps Compile.reflect Compile.value'
-                       Option.sequence Option.sequence_return Option.bind
-                       UnderLets.reify_and_let_binds_base_cps
-                       UnderLets.splice UnderLets.splice_list UnderLets.to_expr
-                       base.interp base.base_interp
-                       base.type.base_beq
-                       type.try_make_transport_cps base.try_make_transport_cps base.try_make_base_transport_cps
-                       PrimitiveProd.Primitive.fst PrimitiveProd.Primitive.snd Datatypes.fst Datatypes.snd
-                    ] in arith_rewrite_head2.
-      (* Finished transaction in 3.967 secs (3.968u,0.s) (successful) *)
+        := make_rewrite_head (@arith_rewrite_head0 var max_const_val do_again t idc) (@arith_pr2_rewrite_rules).
+      (* Tactic call ran for 0.283 secs (0.284u,0.s) (success)
+         Tactic call ran for 79.61 secs (79.612u,0.008s) (success)
+         Tactic call ran for 3.574 secs (3.576u,0.s) (success)
+         Finished transaction in 83.677 secs (83.68u,0.008s) (successful) *)
 
       Local Set Printing Depth 1000000.
       Local Set Printing Width 200.
@@ -2395,14 +2308,35 @@ Z.mul @@ (?x >> 128, ?y >> 128)             --> mulhh @@ (x, y)
       (* Redirect "/tmp/arith_rewrite_head" Print arith_rewrite_head. *)
     End red_arith.
 
+    Section red_arith_with_casts.
+      Context {var : type.type base.type -> Type}
+              (do_again : forall t : base.type, @expr base.type ident (@Compile.value base.type ident var) (type.base t)
+                                                -> @UnderLets.UnderLets base.type ident var (@expr base.type ident var (type.base t)))
+              {t} (idc : ident t).
+
+      Time Definition arith_with_casts_rewrite_head
+        := make_rewrite_head (@arith_with_casts_rewrite_head0 var do_again t idc) (@arith_with_casts_pr2_rewrite_rules).
+
+      Local Set Printing Depth 1000000.
+      Local Set Printing Width 200.
+      Import RewriterPrintingNotations.
+      (* Redirect "/tmp/arith_with_casts_rewrite_head" Print arith_with_casts_rewrite_head. *)
+    End red_arith_with_casts.
+
     Definition RewriteNBE {t} (e : expr.Expr (ident:=ident) t) : expr.Expr (ident:=ident) t
       := @Compile.Rewrite (@nbe_rewrite_head) nbe_default_fuel t e.
     Definition RewriteArith (max_const_val : Z) {t} (e : expr.Expr (ident:=ident) t) : expr.Expr (ident:=ident) t
       := @Compile.Rewrite (@arith_rewrite_head max_const_val) arith_default_fuel t e.
+    Definition RewriteArithWithCasts {t} (e : expr.Expr (ident:=ident) t) : expr.Expr (ident:=ident) t
+      := @Compile.Rewrite (fun var do_again => @arith_with_casts_rewrite_head var) arith_with_casts_default_fuel t e.
     Definition RewriteToFancy
-               (invert_low invert_high : Z (*log2wordmax*) -> Z -> option Z)
+               (invert_low invert_high : Z (*log2wordmax*) -> Z -> @option Z)
                {t} (e : expr.Expr (ident:=ident) t) : expr.Expr (ident:=ident) t
       := @Compile.Rewrite (fun var _ => @fancy_rewrite_head invert_low invert_high var) fancy_default_fuel t e.
+    Definition RewriteToFancyWithCasts
+               (invert_low invert_high : Z (*log2wordmax*) -> Z -> @option Z)
+               {t} (e : expr.Expr (ident:=ident) t) : expr.Expr (ident:=ident) t
+      := @Compile.Rewrite (fun var _ => @fancy_with_casts_rewrite_head (*invert_low invert_high*) var) fancy_with_casts_default_fuel t e.
   End RewriteRules.
 
   Import defaults.
